Simplified counter. Include suggestions by @jakobbotsch and @spitters

execution/theories/Examples/Counter.v
@@ -24,28 +24,34 @@ Section Counter.
   (** The definitions in this section are generalized over the [ChainBase] that specifies the type of addresses and which properties such a type must have *)
   Context {BaseTypes : ChainBase}.
 
+  (** The state is a current counter value and the owner's address *)
   Record State :=
-    mkState { count : Z ;
-              owner : Address }.
+    build_state { count : Z ;
+                  owner : Address }.
 
+  (** The contract accepts two kinds of messages: increment or decrement by some number *)
   Inductive Msg :=
-  | Inc (_ : Z)
-  | Dec (_ : Z).
+  | Inc (i : Z)
+  | Dec (i : Z).
 
-  Definition increment (st : State) (new_balance : Z) :=
-    {| count := st.(count) + new_balance ;
+
+  (** Since a contract is essentially a state transition function, we isolate
+      the functionality corresponding to each kind of message into step functions *)
+  Definition increment (n : Z) (st : State) : State :=
+    {| count := st.(count) + n ;
        owner := st.(owner) |}.
 
-  Definition decrement (st : State) (new_balance : Z) :=
-      {| count := st.(count) - new_balance ;
-         owner := st.(owner) |}.
+  Definition decrement (n : Z) (st : State) : State :=
+    {| count := st.(count) - n ;
+       owner := st.(owner) |}.
 
-  (** The main functionality of the contract *)
+  (** The main functionality of the contract.
+      Dispatches on a message, validates the input and calls the step functions *)
   Definition counter (st : State) (msg : Msg) : option State :=
     match msg with
-    | Inc i => if (0 <? i) then Some (increment st i)
+    | Inc i => if (0 <? i) then Some (increment i st)
               else None
-    | Dec i => if (0 <? i) then Some (decrement st i)
+    | Dec i => if (0 <? i) then Some (decrement i st)
               else None
     end.
 
@@ -68,14 +74,14 @@ Section Counter.
 
   (** Deriving the [Serializable] instances for the state and for the messages *)
   Global Instance State_serializable : Serializable State :=
-  Derive Serializable State_rect<mkState>.
+    Derive Serializable State_rect<build_state>.
 
   Global Instance Msg_serializable : Serializable Msg :=
     Derive Serializable Msg_rect<Inc, Dec>.
 
   (** The counter contract *)
   Program Definition counter_contract : Contract Z Msg State :=
-  build_contract counter_init _ counter_receive _.
+    build_contract counter_init _ counter_receive _.
 
 End Counter.
 
@@ -88,59 +94,22 @@ Section FunctionalProperties.
 
   (** *** Specification *)
 
-  Definition increments (f : State -> option State) (prev_state : State) (n : Z) :=
-    exists next_state, f prev_state = Some next_state
-                /\ next_state.(count) >= prev_state.(count)
-                /\ next_state.(count) = (prev_state.(count) + n).
-
-  Definition decrements (f : State -> option State) (prev_state : State) (n : Z) :=
-    exists next_state, f prev_state = Some next_state
-                /\ next_state.(count) <= prev_state.(count)
-                /\ next_state.(count) = (prev_state.(count) - n).
-
-  (** Counter increments, decrements or fails *)
-  Definition counter_spec (f : State -> option State) (msg : Msg) :=
-    forall state, (exists n, msg = Inc n /\ increments f state n)
-           \/ (exists n, msg = Dec n /\ decrements f state n)
-           \/ f state = None.
-
-  (** *** Proofs of functional correctness properties *)
-  Lemma increment_correct state m :
-    0 < m ->
-    increments (fun s => counter s (Inc m)) state m.
+  (** If the counter call succeeds and returns [next_state] then,
+      depending on a message, it either increments or decrements
+      by the number sent in the corresponding message *)
+  Lemma counter_correct {prev_state next_state msg} :
+  counter prev_state msg = Some next_state ->
+  match msg with
+  | Inc n => prev_state.(count) < next_state.(count)
+             /\ next_state.(count) = prev_state.(count) + n
+  | Dec n => prev_state.(count) > next_state.(count)
+             /\ next_state.(count) = prev_state.(count) - n
+  end.
   Proof.
-    intros Hm.
-    eexists. repeat split.
-    - simpl. rewrite <-Z.ltb_lt in *; now rewrite Hm.
-    - simpl. subst. lia.
-    - simpl. congruence.
-  Qed.
-
-  Lemma decrement_correct state  m :
-    0 < m ->
-    decrements (fun s => counter s (Dec m)) state m.
-  Proof.
-    intros Hm.
-    eexists. repeat split.
-    - simpl. rewrite <-Z.ltb_lt in *; now rewrite Hm.
-    - simpl. subst. lia.
-    - simpl. congruence.
-  Qed.
-
-  Lemma counter_correct (msg : Msg) : counter_spec (fun s => counter s msg) msg.
-  Proof.
-    intros state.
-    destruct msg eqn:Hmsg.
-    + destruct (0 <? z) eqn:Hz.
-      * left. eexists. split;eauto.
-        rewrite Z.ltb_lt in *.
-        now apply increment_correct.
-      * cbn. rewrite Hz;auto.
-    + destruct (0 <? z) eqn:Hz.
-      * right. left. eexists. split;eauto.
-        rewrite Z.ltb_lt in *.
-        now apply decrement_correct.
-      * cbn. rewrite Hz;auto.
+    intros H.
+    all : destruct msg;cbn in *;unfold increment,decrement in *.
+    all : destruct (0 <? i) eqn:Hz;inversion H;cbn in *.
+    all : rewrite Z.ltb_lt in *;split;auto;lia.
   Qed.
 
 End FunctionalProperties.
@@ -152,20 +121,11 @@ Section SafetyProperties.
 
 Context {BaseTypes : ChainBase}.
 
-(** Auxiliary definitions for stating the safety property *)
-Definition counter_state (env : Environment) (address : Blockchain.Address) : option State :=
-match (env_contract_states env address) with
-| Some sv => deserialize sv
-| None => None
-end.
-
 (** Converting a message to a number. Note that the decrements are negative. *)
 Definition opt_msg_to_number (msg : option Msg) :=
   match msg with
-  | Some m => match m with
-             | Inc n => n
-             | Dec n => - n
-             end
+  | Some (Inc i) => i
+  | Some (Dec i) => - i
   | _ => 0
   end.
 
@@ -194,7 +154,7 @@ Lemma counter_safe block_state counter_addr
   env_contracts block_state counter_addr = Some (counter_contract : WeakContract) ->
   exists cstate call_info deploy_info,
     incoming_calls Msg trace counter_addr = Some call_info
-    /\ counter_state block_state counter_addr = Some cstate
+    /\ contract_state block_state counter_addr = Some cstate
     /\ deployment_info _ trace counter_addr = Some deploy_info
     /\ let init_val := deploy_info.(deployment_setup) in
       init_val + sum_inc_dec call_info = cstate.(count).
@@ -203,32 +163,11 @@ Proof.
   + (* deployment *)
     inversion init_some;subst;clear init_some;cbn in *. lia.
   + (* contract call *)
-    unfold receive in *.
-    destruct msg as [msg|];try discriminate.
+    destruct msg as [msg|];try discriminate;cbn in *.
+    destruct (counter _ _) as [cstate|] eqn:counter_some;inversion receive_some;subst.
     (* NOTE: we use the functional correctness here *)
-    specialize (counter_correct msg prev_state) as Cspec.
-    destruct Cspec as [Hinc|[Hdec|Hfail]].
-    * (* increments *)
-      destruct Hinc as (n & Hmsg & Hinc).
-      unfold increments in Hinc.
-      destruct Hinc as (next_cstate & Hnstate & ? & Hadds).
-      unfold counter_receive in *.
-      rewrite Hnstate in receive_some.
-      inversion receive_some;subst;clear receive_some.
-      cbn in *. destruct (0 <? n);inversion Hnstate;subst.
-      rewrite Hadds. rewrite <-IH;auto. unfold sum_inc_dec. lia.
-    *  (* decrements *)
-      destruct Hdec as (n & Hmsg & Hdec).
-      unfold decrements in Hdec.
-      destruct Hdec as (next_cstate & Hnstate & ? & Hsubstracts).
-      unfold counter_receive in *.
-      rewrite Hnstate in receive_some.
-      inversion receive_some;subst;clear receive_some.
-      cbn in *. destruct (0 <? n);inversion Hnstate;subst.
-      rewrite Hsubstracts. rewrite <-IH;auto. unfold sum_inc_dec. lia.
-    * (* fails *)
-      unfold counter_receive in *.
-      now rewrite Hfail in receive_some.
+    specialize (counter_correct counter_some) as Cspec.
+    destruct msg;intuition;unfold sum_inc_dec in *;lia.
   + (* contract self-call *)
     (* NOTE: we know that the self-call is not possible because [counter_receive]
        always returns an empty list of actions. We instantiate the [CallFacts]
@@ -236,12 +175,12 @@ Proof.
        contract address. We will be asked to prove this goal later. *)
     instantiate (CallFacts := fun _ ctx _ => ctx_from ctx <> ctx_contract_address ctx);
       subst CallFacts; cbn in *; congruence.
-  + (* we asked to prove additional assumtions we might have made.
+  + (* we asked to prove additional assumptions we might have made.
      Since we instantiated only [CallFacts], we instantiate other assumptions
      with a trivial proposition *)
     instantiate (AddBlockFacts := fun _ _ _ _ _ _ => True).
     instantiate (DeployFacts := fun _ _ => True).
-    unset_all; subst; cbn in *.
+    unset_all;subst;cbn in *.
     destruct_chain_step; auto.
     destruct_action_eval; auto.
     cbn. intros cstate Hc Hstate.
@@ -249,10 +188,9 @@ Proof.
     assert ((outgoing_acts bstate_from to_addr) = []) as Hempty.
     { apply lift_outgoing_txs_empty with (contract := counter_contract);eauto.
       intros. eapply (receive_produces_no_calls (chain:=chain) (ctx:=ctx));eauto. apply H. }
-    unfold outgoing_acts in *.
-    rewrite queue_prev in *.
-    subst act; cbn in Hempty.
-    destruct_address_eq; cbn in *; auto.
+    unfold outgoing_acts in *. rewrite queue_prev in *.
+    subst act;cbn in Hempty.
+    now destruct_address_eq.
 Qed.
 
 End SafetyProperties.
